%%%%%%%%%%%%%%%%%%%%%%%%%%%%%%%%%%%%%%%%%%%%%%%%%%%%%%%%%%%%%%%
%
% Welcome to Overleaf --- just edit your LaTeX on the left,
% and we'll compile it for you on the right. If you open the
% 'Share' menu, you can invite other users to edit at the same
% time. See www.overleaf.com/learn for more info. Enjoy!
%
%%%%%%%%%%%%%%%%%%%%%%%%%%%%%%%%%%%%%%%%%%%%%%%%%%%%%%%%%%%%%%%


% Inbuilt themes in beamer
\documentclass{beamer}

% Theme choice:
\usetheme{CambridgeUS}

% Title page details: 
\title{Assignment 6} 
\author{Kummitha Jhanavi (CS21BTECH11032)}
\date{\today}
\logo{\large \LaTeX{}}


\begin{document}

% Title page frame
\begin{frame}
    \titlepage 
\end{frame}

% Remove logo from the next slides
\logo{}


% Outline frame
\begin{frame}{Outline}
    \tableofcontents
\end{frame}

\section{Question}
\begin{frame}{Question}
\begin{block}
    
    (a) Show that if y=ax+b,then $\sigma$_{y} =|a|$\sigma$_{\lambda}.
    (b) Find $ \eta$, and $ \sigma$, if y= $\frac{x-\eta_{x}}{\sigma_{x}}$
\end{block}
    
\end{frame}
\section{Solution}
\begin{frame}{Solution}
\begin{block}
    
    (a) \begin{equation}
        \eta_{y} = a \eta_{x} +b
    \end{equation}
    \begin{equation}
        \sigma ^2 _{y} = E({[a x + b -(a \eta_{x}+b)]^2})
    \end{equation}
    \begin{equation}
        \sigma ^2 _{y}= E({a^2(x- \eta_{x})^2}) = a^2\sigma^2_{x}
          \end{equation}
    \begin{equation}
        \sigma_{y} = |a| \sigma_{y}
    \end{equation}
    
    (b) \begin{equation}
        y = \frac{x-\eta_{x}}{\sigma{x}}
    \end{equation}
    \begin{equation}
        E(y) = 0
    \end{equation}
    \begin{equation}
        \sigma^2_{y} = \frac{\sigma^2_{x}}{\sigma^2_{x}}=1
    \end{equation}
    
    
\end{block}
    
\end{frame}




\end{document}
